CoqDoc test push

DList.v
@@ -21,7 +21,7 @@ Module Type ListType.
       | true => (Some 0)
       | false => match (find x comp ls) with
         | None => None
-        | Some n => Some (n+1)
+        | Some n => Some (S n)
         end
       end
     end.
@@ -45,7 +45,7 @@ Module Type ListType.
   Fixpoint len (l:t2) : nat :=
     match l with
     | nil => 0
-    | (cons x' ls) => (len ls) + 1
+    | (cons x' ls) => S (len ls)
     end.
   Fixpoint rev (l:t2) : t2 :=
     match l with
@@ -65,4 +65,224 @@ Module Type ListType.
     | nil => lst
     | (cons (n1,val1) rem) => setMany rem (set n1 val1 lst)
     end.
+
+  Theorem prep_rev : forall a lst, rev (prep a lst) = cons a (rev lst).
+  Proof.
+    intros.
+    induction lst.
+    auto.
+    simpl.
+    rewrite IHlst.
+    simpl.
+    reflexivity.
+  Qed.
+
+  Theorem rev_rev_same : forall lst:t2, rev (rev lst) = lst.
+  Proof.
+    induction lst.
+    auto.
+    simpl.
+    rewrite prep_rev.
+    rewrite IHlst.
+    reflexivity.
+  Qed.
+
+  Theorem get_nil : forall n, get n nil = None.
+  Proof.
+    intros; destruct n; auto.
+  Qed.
+
+  Theorem get_set_avail : forall n v lst, n < (len lst) -> get n (set n v lst) = Some v.
+  Proof.
+    intros.
+    generalize dependent n.
+    induction lst; simpl; intros.
+    inversion H.
+    destruct n; auto.
+    simpl.
+    apply IHlst.
+    apply Sn_Sm_lt_n_m.
+    auto.
+  Qed.
+
+  Theorem get_set_unavail : forall n v lst, ~ (n < (len lst)) -> get n (set n v lst) = None.
+  Proof.
+    induction n.
+    destruct lst; intros.
+    auto.
+    simpl in H. assert False.
+    apply H. apply zero_lt_S_n.
+    inversion H0.
+    intros.
+    destruct lst.
+    auto.
+    simpl.
+    assert (~ (n < len lst)).
+    intro Contra.
+    apply H.
+    simpl.
+    apply n_m_lt_Sn_Sm. assumption.
+    apply IHn.
+    assumption.
+  Qed.
+
+  Theorem find_in_range : forall x cmp lst n1, ( find x cmp lst ) = Some n1 -> n1 < (len lst).
+  Proof.
+    intros.
+    generalize dependent n1.
+    induction lst; intros; inversion H.
+      destruct (cmp x a).
+        inversion H1.
+        simpl.
+        apply zero_lt_S_n.
+        destruct (find x cmp lst).
+          inversion H1.
+          simpl.
+          apply n_m_lt_Sn_Sm.
+          apply IHlst.
+          reflexivity.
+          inversion H1.
+  Qed.    
+
+  Theorem find_set_get : forall x cmp lst n1 v, ( find x cmp lst ) = Some n1 -> get n1 (set n1 v lst) = Some v.
+  Proof.
+    intros.
+    apply find_in_range in H.
+    apply get_set_avail.
+    assumption.
+  Qed.
+
+  Theorem get_set_indep : forall n n' v v' lst, n<>n' -> get n lst = Some v -> get n (set n' v' lst) = Some v.
+  Proof.
+    intros.
+    generalize dependent n.
+    generalize dependent n'.
+    induction lst; intros.
+    destruct n; inversion H0.
+    destruct n; destruct n'.
+      assert False.
+        apply H. reflexivity.
+        inversion H1.
+      simpl. simpl in H0. assumption.
+      simpl. simpl in H0. assumption.
+      simpl. simpl in H0. apply IHlst.
+        intro Contra. apply H. rewrite Contra. reflexivity.
+        assumption.
+  Qed.
+
+  Theorem get_set_dep : forall n n' v v' lst, n=n' -> get n lst = Some v -> get n (set n' v' lst) = Some v'.
+  Proof.
+    intros.
+    generalize dependent n.
+    generalize dependent n'.
+    induction lst; intros.
+    destruct n; inversion H0.
+    destruct n; subst.
+      auto.
+      simpl. apply IHlst; auto.
+  Qed.
+
+  Inductive compRel : (t1->t1->bool) -> t1 -> t1 -> Prop :=
+    | fRel : forall (cmp:(t1->t1->bool)) (inp1:t1) (inp2:t1), (boolCoerced (cmp inp1 inp2)) -> compRel cmp inp1 inp2.
+
+  Theorem compEq : forall (x1 x2:t1) (cmp:t1->t1->bool), (cmp x1 x2 = true) <-> compRel cmp x1 x2.
+  Proof.
+    intros.
+    split; intro.
+      econstructor. rewrite H. constructor.
+      inversion H. inversion H0. reflexivity.
+  Qed.
+
+  Inductive findRel : t1 -> (t1 -> t1 -> bool ) -> t2 -> (@Option nat) -> Prop :=
+    | currFindRel : forall (x x2:t1) (cmp:t1->t1->bool) (rem:t2), compRel cmp x x2 -> findRel x cmp (cons x2 rem) (Some 0)
+    | remFindRel : forall (x x2:t1) (cmp:t1->t1->bool) (rem:t2) (n:nat), ~(compRel cmp x x2) -> findRel x cmp rem (Some n) -> findRel x cmp (cons x2 rem) (Some (S n))
+    | nilFindRelNone : forall (x:t1) (cmp:t1->t1->bool), findRel x cmp nil None
+    | remFindRelNone : forall (x x2:t1) (cmp:t1->t1->bool) (rem:t2), ~(compRel cmp x x2) -> findRel x cmp rem None -> findRel x cmp (cons x2 rem) None.
+
+  Theorem findRelEq : forall (x:t1) (cmp:t1->t1->bool) (lst:t2) (res:@Option nat),(findRel x cmp lst res) <-> (find x cmp lst = res).
+  Proof.
+    induction lst; split; intro.
+    inversion H; simpl; reflexivity.
+    simpl in H; subst; econstructor.
+    inversion H; subst; simpl; remember (cmp x a) as cmpres; destruct cmpres; auto.
+      inversion H5. rewrite <- Heqcmpres in H0. inversion H0.
+      assert(False). apply H4. econstructor. rewrite <- Heqcmpres. econstructor. inversion H0.
+      apply IHlst in H6. rewrite H6. reflexivity.
+      assert(False). apply H4. econstructor. rewrite <- Heqcmpres. econstructor. inversion H0.
+      apply IHlst in H6. rewrite H6. reflexivity.
+    simpl in H; remember (cmp x a) as cmpres; destruct cmpres.
+      subst; econstructor. econstructor. rewrite <- Heqcmpres. econstructor.
+      destruct (find x cmp lst); subst; econstructor; try (intro; inversion H; inversion H0; rewrite <- Heqcmpres in H5; inversion H5); try (eapply IHlst; reflexivity).
+  Qed.
+
+  Inductive getRel : nat -> t2 -> @Option t1 -> Prop :=
+    | zeroGetRel : forall (x:t1) (lst:t2), getRel 0 (cons x lst) (Some x)
+    | succGetRel : forall (n:nat) (x y:t1) (lst:t2), getRel n lst (Some x) -> getRel (S n) (cons y lst) (Some x)
+    | nilGetRelNone : forall (n:nat), getRel n nil None
+    | consGetRelNone : forall (n:nat) (lst:t2) (x:t1), getRel n lst None -> getRel (S n) (cons x lst) None.
+
+  Theorem getRelEq : forall (n:nat) (x:@Option t1) (lst:t2), getRel n lst x <-> get n lst = x.
+  Proof.
+    induction n.
+    split; intro.
+      inversion H; simpl; reflexivity.
+      destruct lst; simpl in H; subst; econstructor.
+    split; intro.
+      inversion H; simpl; auto; apply IHn; auto.
+      destruct lst; simpl in H; subst; try econstructor.
+        remember (get n lst) as gtlst. destruct gtlst; econstructor; eapply IHn; symmetry; assumption.
+  Qed.
+
+  Inductive setRel : nat -> t1 -> t2 -> t2 -> Prop :=
+    | nilSet : forall (n:nat) (x:t1), setRel n x nil nil
+    | currConsSet : forall (x y:t1) (lst:t2), setRel 0 x (cons y lst) (cons x lst)
+    | succConsSet : forall (n:nat) (x y:t1) (lst lst':t2), setRel n x lst lst' -> setRel (S n) x (cons y lst) (cons y lst').
+
+  Theorem setRelEq : forall (n:nat) (x:t1) (lst lst':t2), (set n x lst = lst') <-> (setRel n x lst lst').
+  Proof.
+    intros n x lst.
+    generalize dependent n.
+    generalize dependent x.
+    induction lst; split; intro.
+      destruct n; simpl in H; subst; econstructor.
+      inversion H. destruct n; simpl; reflexivity.
+      destruct n; simpl in H; subst; econstructor. apply IHlst. reflexivity.
+      inversion H. simpl. reflexivity. simpl. subst.
+        assert(set n0 x lst = lst'0). apply IHlst. assumption.
+        rewrite H0. reflexivity.
+  Qed.
+
+  Inductive prepRel : t1 -> t2 -> t2 -> Prop :=
+    | nilPrep : forall (x:t1), prepRel x nil (cons x nil)
+    | consPrep : forall (x y:t1) (rem1 rem2:t2), prepRel x rem1 rem2 -> prepRel x (cons y rem1) (cons y rem2).
+
+  Theorem prepRelEq : forall (x:t1) (lst lst':t2), prep x lst = lst' <-> prepRel x lst lst'.
+  Proof.
+    intros x lst.
+    generalize dependent x.
+    induction lst; split; intro.
+      simpl in H; subst; econstructor.
+      inversion H; subst; simpl; reflexivity.
+      simpl in H. destruct lst'; inversion H. econstructor. apply IHlst. reflexivity.
+      inversion H; subst; simpl. apply IHlst in H4. rewrite H4. reflexivity.
+  Qed.
+
+  Inductive setManyRel : list (nat*t1) -> t2 -> t2 -> Prop :=
+    | nilSetManyRel : forall (lst:t2), setManyRel nil lst lst
+    | consSetManyRel : forall (lst1 lst2 lst3:t2) (x:nat) (v1:t1) (rem:list (nat*t1)),
+                        setRel x v1 lst1 lst2 -> setManyRel rem lst2 lst3 ->
+                        setManyRel (cons (x,v1) rem) lst1 lst3.
+
+  Theorem setManyRelEq : forall (data:list (nat*t1)) (lst1 lst2:t2), setMany data lst1 = lst2 <-> setManyRel data lst1 lst2.
+  Proof.
+    induction data;
+    split; intro.
+      simpl in H. subst; try econstructor.
+      inversion H. simpl. reflexivity.
+      simpl in H. subst. destruct a. remember (set n t lst1) as lst2. econstructor.
+        eapply setRelEq. symmetry. eapply Heqlst2.
+        apply IHdata. reflexivity.
+      inversion H. simpl. apply setRelEq in H2. rewrite H2. apply IHdata. assumption.
+  Qed.
+
 End ListType.
