DvmState.v
@@ -51,7 +51,8 @@ Module ChangeState <: ChangeStateType.
   Definition state := DVMState.
   Definition change := deltaState.
   Declare Module VLIST : ListType with Definition t1 := nat*Val.
-  Fixpoint changeFrame (currf:Frame) (fd:frameDiff) : Frame :=
+
+  Definition changeFrame (currf:Frame) (fd:frameDiff) : Frame :=
     match currf,fd with
     | (frm vals ml pc),(upPC pc2) => frm vals ml pc2
     | (frm vals ml pc),(upVals n v1) => match (VLIST.find (n,v1) compFirst vals) with
@@ -59,9 +60,32 @@ Module ChangeState <: ChangeStateType.
       | None => frm (VLIST.prep (n,v1) vals) ml pc
       end
     end.
+
+  Inductive changeFrameRel : Frame -> frameDiff -> Frame -> Prop :=
+    | upPCRel : forall (vals:list (nat*Val)) (ml:MethodLocation) (pc pc2:ProgramCounter), changeFrameRel (frm vals ml pc) (upPC pc2) (frm vals ml pc2)
+    | upValsRel1 : forall (vals1 vals2:list (nat*Val)) (n n1:nat) (v1:Val) (ml:MethodLocation) (pc:ProgramCounter), VLIST.findRel (n,v1) compFirst vals1 (Some n1) -> VLIST.setRel n1 (n,v1) vals1 vals2 -> changeFrameRel (frm vals1 ml pc) (upVals n v1) (frm vals2 ml pc)
+    | upValsRel2 : forall (vals vals2:list (nat*Val)) (n:nat) (v1:Val) (ml:MethodLocation) (pc:ProgramCounter), VLIST.findRel (n,v1) compFirst vals None -> VLIST.prepRel (n,v1) vals vals2 -> changeFrameRel (frm vals ml pc) (upVals n v1) (frm vals2 ml pc).
+
+  Theorem changeFrameRelEq : forall (f1 f2:Frame) (fd:frameDiff), changeFrame f1 fd = f2 <-> changeFrameRel f1 fd f2.
+  Proof.
+    destruct f1.
+    destruct fd; split; intros.
+      simpl in H.
+      remember (VLIST.find (n, v) compFirst vals) as fres.
+      destruct fres; rewrite <- H. 
+        eapply upValsRel1. eapply VLIST.findRelEq. symmetry. eapply Heqfres. apply VLIST.setRelEq. reflexivity.
+        eapply upValsRel2. eapply VLIST.findRelEq. symmetry. eapply Heqfres. apply VLIST.prepRelEq. reflexivity.
+      inversion H; simpl; apply VLIST.findRelEq in H6; rewrite H6. 
+        apply VLIST.setRelEq in H7. rewrite H7. reflexivity.
+        apply VLIST.prepRelEq in H7. rewrite H7. reflexivity.
+      simpl in H. rewrite <- H. econstructor.
+      inversion H. simpl. reflexivity.
+  Qed.
+
   Declare Module ABLIST : ListType with Definition t1 := arrOrObj.
   Declare Module NLIST : ListType with Definition t1 := nat.
-  Fixpoint mkChange (cst:state) (ch:change) : @Option state :=
+
+  Definition mkChange (cst:state) (ch:change) : @Option state :=
     match cst with
     | dst frms h sh inb outb => match ch with
       | createFrame f => Some (dst (cons f frms) h sh inb outb)
@@ -93,6 +117,58 @@ Module ChangeState <: ChangeStateType.
     | stuck => Some stuck
     | halt => Some halt
     end.
+
+  Inductive mkChangeRel : state -> change -> @Option state -> Prop :=
+    | createFrameRel : forall (frms: list Frame) (f:Frame) (h:Heap) (sh:SHeap) (inb outb:Buffer), mkChangeRel (dst frms h sh inb outb) (createFrame f) (Some (dst (cons f frms) h sh inb outb))
+    | updateFrameRel : forall (frms: list Frame) (f1 f2:Frame) (h:Heap) (sh:SHeap) (inb outb:Buffer) (fd:frameDiff),
+                         (changeFrameRel f1 fd f2) ->
+                         mkChangeRel (dst (cons f1 frms) h sh inb outb) (updateFrame fd) (Some (dst (cons f2 frms) h sh inb outb))
+    | deleteFrameRel : forall (frms: list Frame) (f1:Frame) (h:Heap) (sh:SHeap) (inb outb:Buffer),
+                         mkChangeRel (dst (cons f1 frms) h sh inb outb) deleteFrame (Some (dst frms h sh inb outb))
+    | upHeapRel : forall (frms: list Frame) (lst:list (nat*arrOrObj)) (h h':Heap) (sh:SHeap) (inb outb:Buffer),
+                         ABLIST.setManyRel lst h h' ->
+                         mkChangeRel (dst frms h sh inb outb) (upHeap lst) (Some (dst frms h' sh inb outb))
+    | upSHeapRel : forall (frms: list Frame) (h:Heap) (sh sh':SHeap) (inb outb:Buffer),
+                         mkChangeRel (dst frms h sh inb outb) (upSHeap sh') (Some (dst frms h sh' inb outb))
+    | upInbRel : forall (frms: list Frame) (h:Heap) (sh:SHeap) (curs:Cursor) (clst:list (nat*nat)) (lst lst':list nat) (outb:Buffer),
+                         NLIST.setManyRel clst lst lst' ->
+                         mkChangeRel (dst frms h sh (curs,lst) outb) (upInb clst) (Some (dst frms h sh (curs,lst') outb))
+    | upIncRel : forall (frms: list Frame) (h:Heap) (sh:SHeap) (curs1 curs2:Cursor) (lst:list nat) (outb:Buffer),
+                         mkChangeRel (dst frms h sh (curs1,lst) outb) (upInc curs2) (Some (dst frms h sh (curs2,lst) outb))
+    | upOutbRel : forall (frms: list Frame) (h:Heap) (sh:SHeap) (curs:Cursor) (clst:list (nat*nat)) (lst lst':list nat) (inb:Buffer),
+                         NLIST.setManyRel clst lst lst' ->
+                         mkChangeRel (dst frms h sh inb (curs,lst)) (upOutb clst) (Some (dst frms h sh inb (curs,lst')))
+    | upOutcRel : forall (frms: list Frame) (h:Heap) (sh:SHeap) (curs1 curs2:Cursor) (lst:list nat) (inb:Buffer),
+                         mkChangeRel (dst frms h sh inb (curs1,lst)) (upOutc curs2) (Some (dst frms h sh inb (curs2,lst)))
+    | mkStuckRel : forall (frms: list Frame) (h:Heap) (sh:SHeap) (inb outb:Buffer), mkChangeRel (dst frms h sh inb outb) mkStuck (Some stuck)
+    | mkHaltRel : forall (frms: list Frame) (h:Heap) (sh:SHeap) (inb outb:Buffer), mkChangeRel (dst frms h sh inb outb) mkHalt (Some halt)
+    | updateFrameRel2 : forall (h:Heap) (sh:SHeap) (inb outb:Buffer) (fd:frameDiff),
+                         mkChangeRel (dst nil h sh inb outb) (updateFrame fd) None
+    | deleteFrameRel2 : forall (h:Heap) (sh:SHeap) (inb outb:Buffer),
+                         mkChangeRel (dst nil h sh inb outb) deleteFrame None
+    | stuckRel : forall (ch:change), mkChangeRel stuck ch (Some stuck)
+    | haltRel : forall (ch:change), mkChangeRel halt ch (Some halt).
+
+  Theorem mkChangeRelEq : forall (st:state) (ch:change) (fst:@Option state), mkChange st ch = fst <-> mkChangeRel st ch fst.
+  Proof.
+    intros st ch.
+    generalize dependent st.
+    destruct ch; split; intro;
+      try (destruct st; simpl in H; subst; econstructor);
+      try (inversion H; simpl; reflexivity).
+      destruct st; try destruct frms; try simpl in H; try subst; try econstructor. apply changeFrameRelEq. reflexivity.
+      inversion H; simpl; try reflexivity. apply changeFrameRelEq in H2. subst. reflexivity.
+      destruct st; try destruct frms; simpl in H; subst; econstructor.
+      apply ABLIST.setManyRelEq. reflexivity.
+      inversion H; simpl; try reflexivity. apply ABLIST.setManyRelEq in H2. rewrite H2. reflexivity.
+      destruct st; try destruct inb; simpl in H; subst; try econstructor. apply NLIST.setManyRelEq. reflexivity.
+      inversion H; simpl; try reflexivity; try apply NLIST.setManyRelEq in H2; subst; try reflexivity.
+      destruct st; try destruct outb; simpl in H; subst; try econstructor. apply NLIST.setManyRelEq. reflexivity.
+      inversion H; simpl; try reflexivity; try apply NLIST.setManyRelEq in H2; subst; try reflexivity.
+      destruct st; try destruct inb; simpl in H; subst; try econstructor.
+      destruct st; try destruct outb; simpl in H; subst; try econstructor.
+  Qed.
+
   Fixpoint mkChanges (cst:state) (chs:list change) : @Option state :=
     match chs with
     | nil => Some cst
@@ -101,4 +177,30 @@ Module ChangeState <: ChangeStateType.
       | None => None
       end
     end.
+
+  Inductive mkChangesRel : state -> list change -> (@Option state) -> Prop :=
+    | nilMkChangesRel : forall (s:state), mkChangesRel s nil (Some s)
+    | someMkChangesRel : forall (s1 s2:state) (s3:@Option state) (ch1:change) (chrem:list change),
+                         mkChangeRel s1 ch1 (Some s2) ->
+                         mkChangesRel s2 chrem s3 ->
+                         mkChangesRel s1 (cons ch1 chrem) s3
+    | noneMkChangesRel : forall (s1:state) (ch1:change) (chrem:list change),
+                         mkChangeRel s1 ch1 None ->
+                         mkChangesRel s1 (cons ch1 chrem) None.
+
+  Theorem mkChangesRelEq : forall (st1:state) (st2:@Option state) (chs:list change), mkChanges st1 chs = st2 <-> mkChangesRel st1 chs st2.
+  Proof.
+    intros.
+    generalize dependent st1.
+    generalize dependent st2.
+    induction chs; split; intro.
+      simpl in H; subst; econstructor.
+      inversion H; simpl; reflexivity.
+      simpl in H. remember (mkChange st1 a) as st'. destruct st'.
+        econstructor. eapply mkChangeRelEq. rewrite <- Heqst'. eauto. apply IHchs. assumption.
+        subst. symmetry in Heqst'. apply mkChangeRelEq in Heqst'. constructor. assumption.
+      inversion H; simpl; subst. apply mkChangeRelEq in H3; subst. rewrite H3. apply IHchs. assumption.
+      apply mkChangeRelEq in H4; subst. rewrite H4. reflexivity.
+  Qed.
+
 End ChangeState.
