Eval.v
@@ -14,6 +14,7 @@ Module EVAL <: EVALTYPE.
   Declare Module VLIST : ListType with Definition t1 := Val.
   Declare Module LVLIST : ListType with Definition t1 := (FieldLocation*Val).
   Declare Module SVLIST : ListType with Definition t1 := (FieldLocation*Val).
+
   Fixpoint evalReg (n:nat) (st:DVMState) : @Option Val :=
     match st with
     | dst nil _ _ _ _ => None
@@ -27,11 +28,40 @@ Module EVAL <: EVALTYPE.
     | stuck => None
     | halt => None
     end.
+
+  Inductive evalRegRel : nat -> DVMState -> @Option Val -> Prop :=
+    | nilEvalRegRel : forall (n:nat) (h:Heap) (sh:SHeap) (inb outb:Buffer), evalRegRel n (dst nil h sh inb outb) None
+    | someSomeEvalRegRel : forall (n n' n'':nat) (x:Val) (frem:list Frame) (lst:list (nat*Val)) (m:MethodLocation) (pc:ProgramCounter) (h:Heap) (sh:SHeap) (inb outb:Buffer),
+                      RLIST.findRel (n,(ref null)) compFirst lst (Some n') ->
+                      RLIST.getRel n' lst (Some (n'',x)) ->
+                      evalRegRel n (dst (cons (frm lst m pc) frem) h sh inb outb) (Some x)
+    | someNoneEvalRegRel : forall (n n':nat) (frem:list Frame) (lst:list (nat*Val)) (m:MethodLocation) (pc:ProgramCounter) (h:Heap) (sh:SHeap) (inb outb:Buffer),
+                      RLIST.findRel (n,(ref null)) compFirst lst (Some n') ->
+                      RLIST.getRel n' lst None ->
+                      evalRegRel n (dst (cons (frm lst m pc) frem) h sh inb outb) None
+    | noneEvalRegRel : forall (n:nat) (frem:list Frame) (lst:list (nat*Val)) (m:MethodLocation) (pc:ProgramCounter) (h:Heap) (sh:SHeap) (inb outb:Buffer),
+                      RLIST.findRel (n,(ref null)) compFirst lst None ->
+                      evalRegRel n (dst (cons (frm lst m pc) frem) h sh inb outb) None
+    | stuckEvalRegRel : forall (n:nat), evalRegRel n stuck None
+    | haltEvalRegRel : forall (n:nat), evalRegRel n halt None.
+
+  Theorem evalRegRelEq : forall (n:nat) (st:DVMState) (v1:@Option Val), evalReg n st = v1 <-> evalRegRel n st v1.
+  Proof.
+    split; intro.
+    destruct st; simpl in H; subst; simpl; try (destruct n; simpl; econstructor). 
+    destruct frms; simpl.
+      destruct n; simpl; econstructor.
+      destruct n; simpl; destruct f; simpl.
+      remember (RLIST.find (0, ref null) compFirst vals) as fres; destruct fres; symmetry in Heqfres;
+      apply RLIST.findRelEq in Heqfres; try constructor; auto.
+      remember (RLIST.get n vals) as gres; destruct gres; symmetry in Heqgres; apply RLIST.getRelEq in Heqgres.
+      destruct t.
+
   Fixpoint evalLhs (exp:lhs) (st:DVMState) : @Option Val :=
     match exp,st with
     | (reg n),_ => evalReg n st
-    | (acc n exp),dst _ h _ _ _ => match (evalReg n st) with
-      | Some (ref (lRef lc)) => match (HP.get lc h),(evalRhs exp st) with
+    | (acc n n2),dst _ h _ _ _ => match (evalReg n st) with
+      | Some (ref (lRef lc)) => match (HP.get lc h),(evalReg n2 st) with
         | Some (ar (arr n' lst)),(Some (prim (int n''))) => (VLIST.get n'' lst)
         | _,_ => None
         end
@@ -39,7 +69,7 @@ Module EVAL <: EVALTYPE.
       end
     | (ifield n1 n2),(dst _ h _ _ _) => match (evalReg n1 st) with
       | Some (ref (lRef lc)) => match (HP.get lc h) with
-        | Some (dob (obj n' lst)) => match (LVLIST.find (n2,(ref null)) compFirst lst) with
+        | Some (dob (obj n' n'' lst)) => match (LVLIST.find (n2,(ref null)) compFirst lst) with
           | Some n3 => match (LVLIST.get n3 lst) with
             | Some (n',vl') => Some vl'
             | None => None
