Primitives.v
@@ -10,9 +10,11 @@ Inductive BinaryArithOperator : Type :=
   | bmult : BinaryArithOperator
   | bdiv : BinaryArithOperator
   | bmod : BinaryArithOperator
-  | band : BinaryArithOperator
+(*  | band : BinaryArithOperator
   | bor : BinaryArithOperator
-  | bxor : BinaryArithOperator.
+  | bxor : BinaryArithOperator 
+For later*)
+.
 
 Inductive BinaryCompOperator : Type :=
   | beq : BinaryCompOperator
@@ -42,26 +44,76 @@ End PrimitiveType.
 Module PType <: PrimitiveType.
   Definition t := Prim.
   Definition t_type := PrimType.
+
   Fixpoint toNat (x:t) : nat :=
     match x with
     | boolean n => n
     | char n => n
     | int n => n
     end.
+
+  Inductive toNatRel : t -> nat -> Prop :=
+    | boolToNatRel : forall n:nat, toNatRel (boolean n) n
+    | charToNatRel : forall n:nat, toNatRel (char n) n
+    | intToNatRel : forall n:nat, toNatRel (int n) n.
+
+  Theorem toNatRelEq : forall (x:t) (n:nat), toNat x = n <-> toNatRel x n.
+  Proof.
+    destruct x; split; intro; simpl in H; subst; try econstructor; try (inversion H; simpl; reflexivity).
+  Qed.
+
   Fixpoint fromNat (ty:t_type) (n:nat) : t :=
     match ty with
     | Bool => boolean n
     | Char => char n
     | Int => int n
     end.
+
+  Inductive fromNatRel : t_type -> nat -> t -> Prop :=
+    | boolFromNatRel : forall n:nat, fromNatRel Bool n (boolean n)
+    | charFromNatRel : forall n:nat, fromNatRel Char n (char n)
+    | intFromNatRel : forall n:nat, fromNatRel Int n (int n).
+
+  Theorem fromNatRelEq : forall (ty:t_type) (x:t) (n:nat), fromNat ty n = x <-> fromNatRel ty n x.
+  Proof.
+    destruct ty; split; intro; simpl in H; subst; try econstructor; try inversion H; simpl; reflexivity.
+  Qed.
+
   Fixpoint getType (x:t) : t_type :=
     match x with
     | boolean x => Bool
     | char x => Char
     | int x => Int
     end.
+
+  Inductive getTypeRel : t -> t_type -> Prop :=
+    | boolGetTypeRel: forall n:nat, getTypeRel (boolean n) Bool
+    | charGetTypeRel: forall n:nat, getTypeRel (char n) Char
+    | intGetTypeRel: forall n:nat, getTypeRel (int n) Int.
+
+  Theorem getTypeRelEq : forall (x:t) (ty:t_type), getType x = ty <-> getTypeRel x ty.
+  Proof.
+    destruct x; split; intro; simpl in H; subst; try econstructor; inversion H; simpl; reflexivity.
+  Qed.
+
   Definition cast (ty:t_type) (x:t) : t :=
     fromNat ty (toNat x).
+
+  Inductive castRel : t_type -> t -> t -> Prop:=
+    | castRelConstructor : forall (x1 x2:t) (ty:t_type) (n:nat), toNatRel x1 n -> fromNatRel ty n x2 -> castRel ty x1 x2.
+
+  Theorem castRelEq : forall (ty:t_type) (x1 x2:t), cast ty x1 = x2 <-> castRel ty x1 x2.
+  Proof.
+    intros; split; intro.
+    unfold cast in H.
+      remember (toNat x1) as n.
+      econstructor. eapply toNatRelEq. symmetry. eapply Heqn.
+      apply fromNatRelEq. assumption.
+    inversion H. unfold cast. apply toNatRelEq in H0. subst. apply fromNatRelEq.
+    assumption.
+  Qed.
+
   Definition comp (x1 x2:t) : nat :=
     (toNat x1) - (toNat x2).
+
 End PType.
