Instructions.v
@@ -2,6 +2,7 @@ Add LoadPath "D:\DVM".
 Require Export Eval.
 Require Export Example.
 Require Export Method.
+Require Export DType.
 
 Module Type InstructionType.
   Parameter inst : Type. (* ADT for Instrucion *)
@@ -27,7 +28,7 @@ Module INSTRUCTION <: InstructionType.
     | branch r1 _ r2 _ => (cons r1 (cons r2 nil))
     | move _ r1 => (cons r1 nil)
     | update r1 r2 => (cons r1 (cons r2 nil))
-    | unaryArith _ _ r1 => (cons r1 nil)
+    | unary _ _ r1 => (cons r1 nil)
     | binaryArith _ r1 _ r2 => (cons r1 (cons r2 nil))
     | new _ _ => nil
     | newarr _ _ r1 => (cons r1 nil)
@@ -131,13 +132,136 @@ Module INSTRUCTION <: InstructionType.
       end
     end.
 
-  Definition move (l1:rhs) (n:Register) (curr:DVMState) (p:prg) : list deltaState :=
+  Definition evalMove (l1:rhs) (n:Register) (curr:DVMState) (p:prg) : list deltaState :=
     match (EVAL.evalRhs l1 curr) with
     | Some v1 => [updateFrame (upVals n v1)]
     | _ => match curr with
       | halt => [mkHalt]
       | _ => [mkStuck]
       end
+    end.
+
+  Declare Module HEAP : ListType with Definition t1 := arrOrObj.
+  Declare Module VLIST : ListType with Definition t1 := Val.
+  Declare Module FLIST : ListType with Definition t1 := FieldLocation*Val.
+
+  Definition evalUpdate (l1 l2:rhs) (curr:DVMState) (p:prg) : list deltaState :=
+    match l1,(EVAL.evalRhs l2 curr),curr with
+    | _,_,halt => [mkHalt]
+    | _,_,stuck => [mkStuck]
+    | (l (acc r1 r2)),(Some v1),(dst frms h sh inb outb) => match (EVAL.evalReg r1 curr),(EVAL.evalReg r2 curr) with
+      | (Some (ref (lRef loc1))),(Some (prim p2)) => match (HEAP.get loc1 h),(PType.toNat p2) with
+        | Some (ar (arr n1 vlst)),n2 => match (isle_num n2 n1) with
+          | true => [(upHeap [(loc1,(ar (arr n1 (VLIST.set n2 v1 vlst))))])]
+          | _ => [mkStuck]
+          end
+        | _,_ => [mkStuck]
+        end
+      | _,_ => [mkStuck]
+      end
+    | (l (ifield r1 f1)),(Some v1),(dst frms h sh inb outb) => match (EVAL.evalReg r1 curr) with
+      | Some (ref (lRef loc1)) => match (HEAP.get loc1 h) with
+        | Some (dob (obj c1 c2 lst)) => match (FLIST.find (f1,(ref null)) compFirst lst) with
+          | Some n1 => [upHeap [(loc1,(dob (obj c1 c2 (FLIST.set n1 (f1,v1) lst))))]]
+          | _ => [mkStuck]
+          end
+        | _ => [mkStuck]
+        end
+      | _ => [mkStuck]
+      end
+    | (l (sfield f1)),(Some v1),(dst frms h sh inb outb) => match (FLIST.find (f1,(ref null)) compFirst sh) with
+      | Some n1 => [upSHeap (FLIST.set n1 (f1,v1) sh)]
+      | _ => [mkStuck]
+      end
+    | _,_,_ => [mkStuck]
+    end.
+
+  Definition evalUnary (l1:rhs) (n:Register) (op:UnaryOperator) (curr:DVMState) (p:prg) : list deltaState :=
+    match op,(EVAL.evalRhs l1 curr) with
+    | unot,Some (prim p1) => match isle_num 1 (PType.toNat p1) with
+      | true => evalMove (cs cfalse) n curr p
+      | false => evalMove (cs ctrue) n curr p
+      end
+    | unot,Some (ref null) => evalMove (cs ctrue) n curr p
+    | unot,Some _ => evalMove (cs cfalse) n curr p
+    | unot,None => match curr with
+      | halt => [mkHalt]
+      | _ => [mkStuck]
+      end
+    end.
+
+  Definition evalBinaryArith (l1 l2:rhs) (n:Register) (op:BinaryArithOperator) (curr:DVMState) (p:prg) : list deltaState :=
+    match curr with
+    | halt => [mkHalt]
+    | stuck => [mkStuck]
+    | _ => match (EVAL.evalRhs l1 curr),(EVAL.evalRhs l2 curr) with
+      | Some (prim p1),Some (prim p2) => match op with
+        | badd => evalMove (cs (cnat ((PType.toNat p1) + (PType.toNat p2)))) n curr p
+        | bsub => evalMove (cs (cnat ((PType.toNat p1) - (PType.toNat p2)))) n curr p
+        | bmult => evalMove (cs (cnat ((PType.toNat p1) * (PType.toNat p2)))) n curr p
+        | bdiv => evalMove (cs (cnat (div (PType.toNat p1) (PType.toNat p2)))) n curr p
+        | bmod => evalMove (cs (cnat (mod (PType.toNat p1) (PType.toNat p2)))) n curr p
+        end
+      | _,_ => [mkStuck]
+      end
+    end.
+
+  Definition evalNew (n:Register) (cl:ClassLocation) (curr:DVMState) (p:prg) : list deltaState :=
+    match curr with
+    | stuck => [mkStuck]
+    | halt => [mkHalt]
+    | (dst _ h _ _ _) => match (TYPE.createObject p (r (c cl)) h) with
+      | Some (upHeap (cons (lc1,vl1) nil)) => (cons (upHeap (cons (lc1,vl1) nil)) (cons (updateFrame (upVals n (ref (lRef lc1)))) nil) )
+      | _ => [mkStuck]
+      end
+    end.
+
+  Definition evalNewArray (n:Register) (t:type) (l:rhs) (curr:DVMState) (p:prg) : list deltaState :=
+    match curr,(EVAL.evalRhs l curr) with
+    | stuck,_ => [mkStuck]
+    | halt,_ => [mkHalt]
+    | (dst _ h _ _ _),(Some v1) => match (EVAL.evalRhs l curr) with
+      | Some (prim p) => match (TYPE.createArray t (PType.toNat p) h) with
+        | Some (upHeap (cons (lc1,vl1) nil)) => (cons (upHeap (cons (lc1,vl1) nil)) (cons (updateFrame (upVals n (ref (lRef lc1)))) nil) )
+        | _ => [mkStuck]
+        end
+      | _ => [mkStuck]
+      end
+    | _,_ => [mkStuck]
+    end.
+
+  Definition evalCast (n:Register) (t:type) (l:rhs) (curr:DVMState) (p:prg) : list deltaState :=
+    match curr,(EVAL.evalRhs l curr) with
+    | halt,_ => [mkHalt]
+    | stuck,_ => [mkStuck]
+    | (dst frms h sh inb outb),(Some v1) => match v1 with
+      | (ref (lRef loc1)) => match (TYPE.cast p t loc1 h) with
+        | Some (upHeap (cons (l1,ob1) nil)) => (cons (upHeap (cons (l1,ob1) nil)) (cons (updateFrame (upVals n (ref (lRef l1)))) nil))
+        | _ => [mkStuck]
+        end
+      | _ => [mkStuck]
+      end
+    | _,_ => [mkStuck]
+    end.
+
+  Declare Module NLIST:ListType with Definition t1:=nat.
+
+  Definition evalRead (n:Register) (curr:DVMState) (p:prg) : list deltaState :=
+    match curr with
+    | halt => [mkHalt]
+    | stuck => [mkStuck]
+    | (dst frms h sh (crs,lst) outb) => match (NLIST.get crs lst) with
+      | Some num => cons (upInc (S crs)) (cons (updateFrame (upVals n (prim (int num)))) nil)
+      | None => [mkStuck]
+      end
+    end.
+
+  Definition evalWrite (r1:rhs) (curr:DVMState) (p:prg) : list deltaState :=
+    match curr,(EVAL.evalRhs r1 curr) with
+    | halt,_ => [mkHalt]
+    | stuck,_ => [mkStuck]
+    | (dst frms h sh inb (crs,lst)),(Some (prim p1)) => [(upOutc (S crs));(upOutb [(crs,(PType.toNat p1))])]
+    | _,_ => [mkStuck]
     end.
 
 End INSTRUCTION.
