Program.v
@@ -10,16 +10,20 @@ End ProgramType.
 
 Module PROGRAM <: ProgramType.
   Definition prg := Program.
+  
   Definition getMethods (p:prg) := 
     match p with
     | (prog cnl mnl clst flst mlst) => mlst
     end.
+
   Definition getClasses (p:prg) := 
     match p with
     | (prog cnl mnl clst flst mlst) => clst
     end.
+
   Definition getFields (p:prg) := 
     match p with
     | (prog cnl mnl clst flst mlst) => flst
     end.
+
 End PROGRAM.
