makefile
@@ -13,8 +13,18 @@ Files:=Helpers.v\
 
 run:
 	$(COQBIN)coqc
-	
-	
-coqc Helpers.v Primitives.v DList.v	Defs.v Program.v DvmState.v Method.v Eval.v Type.v Example.v Instructions.v
 
 
+for compiling from inside subdirectory
+
+coqc ..\CoqDVM.v ..\Helpers.v ..\Primitives.v ..\DList.v ..\Defs.v ..\Program.v ..\DvmState.v ..\Method.v ..\Eval.v ..\DType.v ..\Example.v ..\Instructions.v
+
+for html doc
+
+coqdoc --no-lib-name --toc --html ..\CoqDVM.v ..\Helpers.v ..\Primitives.v ..\DList.v ..\Defs.v ..\Program.v ..\DvmState.v ..\Method.v ..\Eval.v ..\DType.v ..\Example.v ..\Instructions.v
+
+
+coqdoc --no-lib-name --toc --tex ..\CoqDVM.v ..\Helpers.v ..\Primitives.v ..\DList.v ..\Defs.v ..\Program.v ..\DvmState.v ..\Method.v ..\Eval.v ..\DType.v ..\Example.v ..\Instructions.v
+
+
+coqdoc --no-lib-name --toc --pdf ..\CoqDVM.v ..\Helpers.v ..\Primitives.v ..\DList.v ..\Defs.v ..\Program.v ..\DvmState.v ..\Method.v ..\Eval.v ..\DType.v ..\Example.v ..\Instructions.v
